inorder tree traversal

examples/bintree.v
@@ -4,6 +4,7 @@ From mathcomp Require Import eqtype seq ssrnat.
 From fcsl Require Import axioms pred.
 From fcsl Require Import pcm unionmap heap autopcm automap.
 From HTT Require Import model heapauto.
+From HTT Require Import llist.
 Set Implicit Arguments.
 Unset Strict Implicit.
 Unset Printing Implicit Defensive.
@@ -15,8 +16,13 @@ Inductive tree A := Leaf | Node of (tree A) & A & (tree A).
 
 Fixpoint size_tree {A} (t : tree A) : nat :=
   if t is Node l _ r
-    then size_tree l + size_tree r + 1
+    then (size_tree l + size_tree r).+1
   else 0.
+
+Fixpoint inorder {A} (t : tree A) : seq A :=
+  if t is Node l x r
+    then inorder l ++ x :: inorder r
+  else [::].
 
 (* Tree predicate *)
 
@@ -91,7 +97,7 @@ Program Definition treesize p :
                        Do (if p == null then ret s
                            else l <-- !p;
                                 r <-- !(p.+ 2);
-                                ls <-- go(l, s);
+                                ls <-- go (l, s);
                                 go (r, ls + 1)))
       in len (p, 0)).
 Next Obligation.
@@ -100,13 +106,62 @@ move=>_ go _ p s /= _ [t][] i /= H; case: eqP H=>[->|/eqP Ep] H.
 case: (treep_cont Ep H)=>l[a][r][l'][r'][_][{t H}-> {i}-> [hl][hr][-> Hl Hr]] /=.
 do 2!step.
 apply: [stepX l]@hl=>//= _ hl' [/eqP -> Hl'].
-apply: [gX r]@hr=>//= _ hr' [/eqP -> Hr'] V.
-split; first by rewrite -!addnA 2!eqn_add2l addnC.
-exists l', r', (hl' \+ hr'); split=>//.
-by exists hl', hr'.
+apply: [gX r]@hr=>//= _ hr' [/eqP -> Hr'] _.
+split; first by rewrite -addnA add1n -addnA addnS.
+by exists l', r', (hl' \+ hr'); split=>//; exists hl', hr'.
 Qed.
 Next Obligation.
 by move=>/= p [t][] i /= H; apply: [gE t].
+Qed.
+
+(* Tree inorder traversal *)
+
+Opaque insert new.
+
+Definition inordertravT : Type := forall (ps : ptr * ptr),
+  {(t : tree A) (l : seq A)},
+     STsep (treep ps.1 t # lseq ps.2 l,
+           [vfun s h => h \In treep ps.1 t # lseq s (inorder t ++ l)]).
+
+Program Definition inordertrav p :
+  {t : tree A}, STsep (treep p t,
+                      [vfun s h => h \In treep p t # lseq s (inorder t)]) :=
+  Do (let loop := Fix (fun (go : inordertravT) '(p, s) =>
+                       Do (if p == null then ret s
+                           else l <-- !p;
+                                a <-- !(p.+ 1);
+                                r <-- !(p.+ 2);
+                                s1 <-- go (r, s);
+                                s2 <-- @insert A s1 a;
+                                go (l, s2)))
+      in n <-- new A;
+         loop (p, n)).
+Next Obligation.
+move=>_ go _ p s _ /= [t][xs][] _ /= [h1][h2][-> H1 H2].
+case: eqP H1=>[->|/eqP Ep] H1.
+- step=>V; case: (treep_null (validL V) H1)=>->->/=.
+  by exists Unit, h2.
+case: (treep_cont Ep H1)=>l[a][r][l'][r'][_][{t H1}-> {h1}-> [hl][hr][-> Hl Hr]] /=.
+do 3!step.
+apply: [stepX r, xs]@(hr \+ h2)=>//=; first by move=>_; exists hr, h2.
+move=>s1 _ [hr'][hs][-> Hr' Hs].
+apply: [stepX (inorder r ++ xs)]@hs=>//= pa _ [s2][h'][-> H'].
+apply: [gX l, (a::inorder r ++ xs)]@(hl \+ pa :-> a \+ pa.+ 1 :-> s2 \+ h')=>//=.
+- move=>_; exists hl, (pa :-> a \+ (pa.+ 1 :-> s2 \+ h')); split=>//=.
+  - by rewrite !joinA.
+  by rewrite /lseq /=; exists s2, h'.
+move=>s3 _ [hl''][hs'][-> Hl'' Hs'] _.
+exists (p :-> l' \+ (p.+ 1 :-> a \+ (p.+ 2 :-> r' \+ (hl'' \+ hr')))), hs'; split.
+- by rewrite [RHS](pullX (hl'' \+ hs' \+ hr')) [LHS](pullX (hl'' \+ hs' \+ hr')).
+- by exists l', r', (hl'' \+ hr'); split=>//; exists hl'', hr'.
+by rewrite -catA.
+Qed.
+Next Obligation.
+move=>/= p [t][] i /= H.
+rewrite -(unitL i); apply: [stepR]@Unit=>//= _ _ [->->]; rewrite unitL.
+apply: [gE t, [::]]=>/=.
+- by exists i, Unit; split=>//; rewrite unitR.
+by case=>//= s m _; rewrite cats0.
 Qed.
 
 End Tree.
